---
title: "Maths Formula Compendium"
description: "A complete list of high school math formulaes"
lead: ""
date: 2022-01-25T14:41:39+01:00
lastmod: 2022-01-25T14:41:39+01:00
draft: false
images: []
type: docs
menu:
  etc:
    parent: "maths"
weight: 1
toc: true
---

## Trigonometry

<div style="overflow-x:auto;">

| Name | $0\degree$ | $30\degree (\frac{\pi}{6})$ | $45\degree (\frac{\pi}{4})$ | $60\degree (\frac{\pi}{3})$ | $90\degree (\frac{\pi}{2})$ | $120\degree (\frac{2\pi}{3})$ | $135\degree (\frac{3\pi}{4})$ | $150\degree (\frac{5\pi}{6})$ | $180\degree (\pi)$ |
| --- | --- | --- | --- | --- | --- | --- | --- | --- | --- |
| $\sin$ | $0$ | $\frac{1}{2}$ | $\frac{1}{\sqrt{2}}$ | $\frac{\sqrt{3}}{2}$ | $1$ | $\frac{\sqrt{3}}{2}$ | $\frac{1}{\sqrt{2}}$ | $\frac{1}{2}$ | $0$ |
| $\cos$ | $1$ | $\frac{\sqrt{3}}{2}$ | $\frac{1}{\sqrt{2}}$ | $\frac{1}{2}$ | $0$ | $-\frac{1}{2}$ | $-\frac{1}{\sqrt{2}}$ | $-\frac{\sqrt{3}}{2}$ | $-1$ |
| $\tan$ | $0$ | $\frac{1}{\sqrt{3}}$ | $1$ | $\sqrt{3}$| $\infin$ | $-\sqrt{3}$ | $-1$ | $-\frac{1}{\sqrt{3}}$ | $0$ |
| $\cot$ | $\infin$ | $\sqrt{3}$ | $1$ | $\frac{1}{\sqrt{3}}$ |$0$ | $-\frac{1}{\sqrt{3}}$ | $-1$ | $\sqrt{3}$ | $-\infin$ |
| $\sec$ | $1$ | $\frac{2}{\sqrt{3}}$ | $\sqrt{2}$ |$ 2 $| $\infin$ | $-2$ | $-\sqrt{2}$ | $-\frac{2}{\sqrt{3}}$ | $-1$ |
| $\cosec$ | $\infin$ | $2$ | $\sqrt{2}$ | $\frac{2}{\sqrt{3}}$ | $1$ | $\frac{2}{\sqrt{3}}$ | $\sqrt{2}$ | $2$ | $\infin$ |
</div>

## Inverse Trigonometry

|  | Domain (value) ($x$) | Range (Angle) ($\theta$) |
| --- | --- | --- |
| $sin^{-1}x$ | $[-1,1]$ | $[-\pi/2, \pi/2]$ |
| $\cos^{-1}x$ | $[-1. 1]$ | $[0, \pi]$ |
| $\tan^{-1}x$ | $R$ | $(-\pi/2, \pi/2)$ |
| $\cot^{-1}x$ | $R$ | $(0, \pi)$ |
| $\sec^{-1}x$ | $R- (-1, 1)$ | $[0, \pi-\{\pi/2\}$ |
| $\cosec^{-1}x$ | $R-(-1, 1)$ | $[-\pi/2, \pi/2] - \{0\}$ |

| **Property 1** | **Property 2** | 
| --- | --- | 
| $\sin^{-1}(\sin\theta) = \theta$     | $\sin(\sin^{-1}x) = x$     |
| $\cos^{-1}(\cos\theta) = \theta$     | $\cos(\cos^{-1}x) = x$     |
| $\tan^{-1}(\tan\theta) = \theta$     | $\tan(\tan^{-1}x) = x$     |
| $\cosec^{-1}(\cosec\theta) = \theta$ | $\cosec(\cosec^{-1}x) = x$ |
| $\sec^{-1}(\sec\theta) = \theta$     | $\sec(\sec^{-1}x) = x$     |
| $\cot^{-1}(\cot\theta) = \theta$     | $\cot(\cot^{-1}x) = x$     |

| **Property 3** | |
| --- | --- |
| $sin^{-1}(-x) = -\sin^{-1}{x}$     | $cos^{-1}(-x) \pi -\cos^{-1}{x}$ |
| $tan^{-1}(-x) = -\tan^{-1}{x}$     | $cot^{-1}(-x) \pi -\cot^{-1}{x}$ |
| $cosec^{-1}(-x) = -\cosec^{-1}{x}$ | $sec^{-1}(-x) \pi -\sec^{-1}{x}$ |

| **Property 4** |
| ---  |
| $sin^{-1}(\frac{1}{x}) = \cosec^{-1}x$ |
| $cos^{-1}(\frac{1}{x}) = \sec^{-1}x$   |
| $tan^{-1}(\frac{1}{x}) = \cot^{-1}x$   |

| **Property 5** |
| --- | 
| $sin^{-1}x + \cos ^{-1}x = \frac{\pi}{2}$   |
| $tan^{-1}x + \cot ^{-1}x = \frac{\pi}{2}$   |
| $sec^{-1}x + \cosec ^{-1}x = \frac{\pi}{2}$ |

| **Property 6** |  
| --- | 
| $\sin^{-1}x + \sin^{-1}y = \sin^{-1} \big(x\sqrt{1-y^2} + y\sqrt{1-x^2}\big)$ | 
| $\sin^{-1}x - \sin^{-1}y = \sin^{-1} \big(x\sqrt{1-y^2} - y\sqrt{1-x^2}\big)$ | 

| **Property 7** |
| --- |
| $\cos^{-1}x + \cos^{-1}y = \cos^{-1} \big(xy - \sqrt{1-x^2} \sqrt{1-y^2}\big)$ |
| $\cos^{-1}x - \cos^{-1}y = \cos^{-1} \big(xy + \sqrt{1-x^2} \sqrt{1-y^2}\big)$ |

| **Property 8** |
| --- |
| $\tan^{-1}x - \tan^{-1}{y} = \tan^{-1}\Big(\frac{x+y}{1-xy}\Big)$ |
| $\tan^{-1}x + \tan^{-1}{y} = \tan^{-1}\Big(\frac{x-y}{1+xy}\Big)$ |

**Property 9**

$2\sin^{-1}x = 2 \sin^{-1}(\theta/2)$

$3\sin^{-1}x = \sin^{-1}(3x-4x^2)$

$2\cos^{-1}x = \cos^{-1}(2x^2-1)$

$3\cos^{-1}x = \cos^{-1}(4x^3 -3x)$

<div>
$$
2 \tan^{-1}x = \tan^{-1}\Big(\frac{2x}{1-x^2}\Big) \\ 3\tan^{-1}x = \tan^{-1}\Big(\frac{3x-x^2}{1-3x^2}\Big)
$$
</div>

**Property 10**

$$
2\tan^{-1}x = \begin{cases}\sin^{-1}\Big(\frac{2x}{1+x^2}\Big)\\\cos^{-1}\Big(\frac{1-x^2}{1+x^2}\Big)\end{cases}
$$

$1-\cos\theta = 2 \sin^2(\theta/2)$

$1+ \cos\theta = 2\,\cos^2(\theta/2)$

$\sin\theta = 2\sin(\theta/2)\cos(\theta/2)$

$2\sin^{-1}x + \sin^{-1}(-x) = \cos^{1}x$

<div>
$$
\begin{split}\cos2\theta &= \cos^2\theta - \sin^2\theta \\& = 2\cos^2\theta -1 \\ &= 1 - 2\sin^2\theta \end{split}
$$
</div>

{{< panel title="Expression and Substitution" >}}

| Expression | Substitution | Substitution |
| --- | --- | --- |
| $a^2 + x^2$ | $x = a\tan\theta$ | $x = a\cot\theta$ |
|$a^2-x^2$ | $x=a\sin\theta$ | $x=a\cos\theta$ |
|$x^2-a^2$ | $x=a\sec\theta$ | $x=a\cosec\theta$ |
|$\frac{a-x}{a+x}$ | $x=a\cos2\theta$ | |
|$\frac{a^2+x^2}{a^2-x^2}$ | $x=a^2\cos2\theta$ |  |
{{< /panel >}}

## Line Equations

1. $ax + by + c=0$
    
    $m = -a/b$
        
2. One Point form of line 
    
    $$
    y - y_1 = m (x-x_1)
    $$
    
3. Two point form of line
    
    $$
    y-y_1 = \frac{y_2-y_1}{x_2-x_1}{x-x_1}
    $$
    
4. Intercept Form of line

    $$
    \frac{x}{a} + \frac{y}{b} = 1
    $$

{{< figure src="/images/etc/maths/Intercept_form.svg">}}

5. Normal form of line

    $$
    x\cos \theta + y\sin\theta = P
    $$

  {{< figure src="/images/etc/maths/Normal_Form.svg">}}

6. Point Slope form
    
    
    
    

    $$
    y = mx+ c
    \\\\
    \text{Where $m$ is slope of line defined as  } m = \frac{y_2 - y_1}{x_2 - x_1}
    $$

    {{< figure src="/images/etc/maths/Point_SLope_form.svg">}}

### Distance of a point from a line

$$
\text{Dist}_{PA}= \Bigg|{\frac{ax_1 + by_1 + c}{\sqrt{a^2+b^2}}}\Bigg|
$$

{{< figure src="/images/etc/maths/distance_of_a_point_from_a_line.svg">}}

### Distance between two lines

$y = mx + c_1 \qquad y= mx+c_2$

$$
\text{d} = \Bigg| \frac{c_1 - c_2}{\sqrt{1+m^2}}\Bigg| = \Bigg|\frac{c_1 - c_2}{\sqrt{a^2+b^2}}\Bigg|
$$

### Angle between two lines

Where $m_1$ and $m_2$ are slopes of two lines.

$$
\tan\theta = \frac{m_2 - m_1}{1+m_2m_1}
$$

- If line $l_1$ and $l_2$ are orthogonal to each other, then. $m_1m_2 = -1$
- Collinearity of points
    
    Slope of $AB$ = Slope of $AC$

{{< figure src="/images/etc/maths/Collinearity.svg">}}

## Shapes CSA(Curved Surface Area), T(Total)SA, and volume

### Frustum

$\text{CSA} = \pi l (r_1+ r_2)$

$\text{TSA} = \pi r_1^2 + \pi r_2^2 + \pi l(r_1+r_2)$

$\text{Volume} = \frac{1}{3}\pi h (r_1^2 + r_2^2 + r_1r_2)$ 

where   $l= \sqrt{h^2+(r_1-r_2)^2}$

{{< figure src="/images/etc/maths/frustum.png">}}

## Adjoint and Inverse
| | | 
| --- | --- | 
| $A(\text{adj} A) = \|A\| I_n = (\text{adj}) A$ | 
| $A^{-1} = \frac{1}{\|A\|} (\text{adj} A)$      | $\|\text{adj} A\| = \|A\|^{n-1}$ |
| $(A^\top)^{-1} = (A^{-1})^\top$                | $\text{adj} \space(adj A) = \|A\|^{n-2} A$ |
| $\|A \enspace adj A\| = \|A\|^{n}$             | $\|\text{adj} \space(adj A)\| = \|A\|^{(n-1)^{2}}$ |
| | 
| $\|A^\top\| = \|A\| $| 
| $AA^{-1} = I_n$| 
| $(A^{-1})^{-1} = A$| 
| $(AB)^{-1} = B^{-1}A^{-1}$| 
| $\text{adj}\space AB = (\text{adj} B)(\text{adj} A)$| 
| $\|AB\| = \|A\| \|B\|$|
| $\text{adj}A^\top = (\text{adj} A)\top$|
| $\|KA\| = K^n \|A\|$| 
| $AA^{-1}=I$| 
| $A^{-1}I = A^{-1}$| 

## Finding Log 
1. Given we need to find $\log$ of $\log 15.27$

    - Move the decimal after 1st digit and introduce power of 10.
    
    $$
    \log \textcolor{#f56c42}1.\textcolor{#f56c42}5\textcolor{#ad42f5}2\textcolor{#f542bc}7 \times 10^{\textcolor{#42f5f2}1}
    $$

    When the decimal is moved in left/right:
    $$
    (-)\medspace \overrightarrow{\text{introduce negative powers}} \qquad \overleftarrow{\text{introduce positive powers}} \medspace(+)
    $$

2. Look for $\textcolor{#f56c42}{15}$<sup>th</sup> row and column with label $\textcolor{#ad42f5}2$. which is $\bold{\textcolor{#07fc03}{1818}}$.

3. Add *Mean difference* from column $\textcolor{#f542bc}7$ in the corresponding row. which is $\textcolor{#07fc03}{20}$

    $$
    1818 + 20 = \bold{\textcolor{#07fc03}{1838}}
    $$

4. Write the exponent, insert decimal and write the value calculated in Step 3.

    $$
    \textcolor{#42f5f2}1.\textcolor{#07fc03}{1838}
    $$

5. So $\log 15.27 = \bold{\textcolor{#07fc03}{1.1838}}$

## Finding AntiLog
1. Given we need to find Antilog of $15.5932$
    $$
    \log k = 15.5932 \\\\
    k = Antilog (\medspace \textcolor{#42f5f2}{15}\textcolor{#f56c42}{.59}\textcolor{#ad42f5}3\textcolor{#f542bc}2\medspace)
    $$

2. Look for $0\textcolor{#f56c42}{.59}$<sup>th</sup> row and column with label $\textcolor{#ad42f5}3$. Which is $\bold{\textcolor{#07fc03}{3917}}$.

3. Add *Mean difference* from column $\textcolor{#f542bc}2$ to previous result. Which is $\textcolor{#07fc03}2$

    $$
    3917 + 2 = \bold{\textcolor{#07fc03}{3919}}
    $$

4. Add $1$ to *characteristic* $\textcolor{#42f5f2}{15} = \textcolor{#07fc03}{16}$ and add  insert the decimal from left calculated in step 2. That means we need to add decimal after $\textcolor{#07fc03}{16}$<sup>th</sup> position

    $$
    3919\enspace0000\enspace0000\enspace000 .\\\\
    \implies k = \bold{\textcolor{#07fc03}{3.919\times10^{15}}}
    $$

{{< alert title="Quickly write the exponential form">}}
Since, we want to put decimal just after 1<sup>st</sup> digit. We need to move decimal from 16<sup>th</sup> position to right after 1<sup>st</sup> digit; which will introduce +ve powers. ($16 -1 = \textcolor{#07fc03}{15}$). Since we moved 15 positions left.

$3.919 \times 10^{\textcolor{#07fc03}{15}}$
{{< /alert >}}
