---
title: "Maths Formula Compendium"
description: "A complete list of high school math formaulaes"
lead: ""
date: 2022-01-25T14:41:39+01:00
lastmod: 2022-01-25T14:41:39+01:00
draft: false
images: []
type: docs
menu:
  etc:
    parent: "maths"
weight: 100
toc: true
---

## Trigonometry

| Name | $0\degree$ | $30\degree (\frac{\pi}{6})$ | $45\degree (\frac{\pi}{4})$ | $60\degree (\frac{\pi}{3})$ | $90\degree (\frac{\pi}{2})$ | $120\degree (\frac{2\pi}{3})$ | $135\degree (\frac{3\pi}{4})$ | $150\degree (\frac{5\pi}{6})$ | $180\degree (\pi)$ |
| --- | --- | --- | --- | --- | --- | --- | --- | --- | --- |
| $\sin$ | $0$ | $\frac{1}{2}$ | $\frac{1}{\sqrt{2}}$ | $\frac{\sqrt{3}}{2}$ | $1$ | $\frac{\sqrt{3}}{2}$ | $\frac{1}{\sqrt{2}}$ | $\frac{1}{2}$ | $0$ |
| $\cos$ | $1$ | $\frac{\sqrt{3}}{2}$ | $\frac{1}{\sqrt{2}}$ | $\frac{1}{2}$ | $0$ | $-\frac{1}{2}$ | $-\frac{1}{\sqrt{2}}$ | $-\frac{\sqrt{3}}{2}$ | $-1$ |
| $\tan$ | $0$ | $\frac{1}{\sqrt{3}}$ | $1$ | $\sqrt{3}$| $\infin$ | $-\sqrt{3}$ | $-1$ | $-\frac{1}{\sqrt{3}}$ | $0$ |
| $\cot$ | $\infin$ | $\sqrt{3}$ | $1$ | $\frac{1}{\sqrt{3}}$ |$0$ | $-\frac{1}{\sqrt{3}}$ | $-1$ | $\sqrt{3}$ | $-\infin$ |
| $\sec$ | $1$ | $\frac{2}{\sqrt{3}}$ | $\sqrt{2}$ |$ 2 $| $\infin$ | $-2$ | $-\sqrt{2}$ | $-\frac{2}{\sqrt{3}}$ | $-1$ |
| $\cosec$ | $\infin$ | $2$ | $\sqrt{2}$ | $\frac{2}{\sqrt{3}}$ | $1$ | $\frac{2}{\sqrt{3}}$ | $\sqrt{2}$ | $2$ | $\infin$ |

## Inverse Trigonometry

|  | Domain (value) ($x$) | Range (Angle) ($\theta$) |
| --- | --- | --- |
| $sin^{-1}x$ | $[-1,1]$ | $[-\pi/2, \pi/2]$ |
| $\cos^{-1}x$ | $[-1. 1]$ | $[0, \pi]$ |
| $\tan^{-1}x$ | $R$ | $(-\pi/2, \pi/2)$ |
| $\cot^{-1}x$ | $R$ | $(0, \pi)$ |
| $\sec^{-1}x$ | $R- (-1, 1)$ | $[0, \pi-\{\pi/2\}$ |
| $\cosec^{-1}x$ | $R-(-1, 1)$ | $[-\pi/2, \pi/2] - \{0\}$ |

**Property 1** 

- $\sin^{-1}(\sin\theta) = \theta$
- $\cos^{-1}(\cos\theta) = \theta$
- $\tan^{-1}(\tan\theta) = \theta$
- $\cosec^{-1}(\cosec\theta) = \theta$
- $\sec^{-1}(\sec\theta) = \theta$
- $\cot^{-1}(\cot\theta) = \theta$

**Property 2**

- $\sin(\sin^{-1}x) = x$
- $\cos(\cos^{-1}x) = x$
- $\tan(\tan^{-1}x) = x$
- $\cosec(\cosec^{-1}x) = x$
- $\sec(\sec^{-1}x) = x$
- $\cot(\cot^{-1}x) = x$

**Property 3**

- $sin^{-1}(-x) = -\sin^{-1}{x}$
- $tan^{-1}(-x) = -\tan^{-1}{x}$
- $cosec^{-1}(-x) = -\cosec^{-1}{x}$

- $cos^{-1}(-x) \pi -\cos^{-1}{x}$
- $cot^{-1}(-x) \pi -\cot^{-1}{x}$
- $sec^{-1}(-x) \pi -\sec^{-1}{x}$

**Property 4**

- $sin^{-1}(\frac{1}{x}) = \cosec^{-1}x$
- $cos^{-1}(\frac{1}{x}) = \sec^{-1}x$
- $tan^{-1}(\frac{1}{x}) = \cot^{-1}x$

**Property 5**

- $sin^{-1}x + \cos ^{-1}x = \frac{\pi}{2}$
- $tan^{-1}x + \cot ^{-1}x = \frac{\pi}{2}$
- $sec^{-1}x + \cosec ^{-1}x = \frac{\pi}{2}$

**Property 6**

- $\sin^{-1} + \sin^{-1}y = \sin^{-1} \big(x\sqrt{1-y^2} + y\sqrt{1-x^2}\big)$
- $\sin^{-1} - \sin^{-1}y = \sin^{-1} \big(x\sqrt{1-y^2} - y\sqrt{1-x^2}\big)$

**Property 7**

- $\cos^{-1} + \cos^{-1}y = \cos^{-1} \big(xy - \sqrt{1-x^2} \sqrt{1-y^2}\big)$
- $\cos^{-1} - \cos^{-1}y = \cos^{-1} \big(xy + \sqrt{1-x^2} \sqrt{1-y^2}\big)$

**Property 8**

- $\tan^{-1} - \tan^{-1}{y} = \tan^{-1}\Big(\frac{x+y}{1-xy}\Big)$
- $\tan^{-1} + \tan^{-1}{y} = \tan^{-1}\Big(\frac{x-y}{1+xy}\Big)$

 **Property 9**

- $2\sin^{-1}x = 2 \sin^{-1}(\theta/2)$
- $3\sin^{-1}x = \sin^{-1}(3x-4x^2)$

- $2\cos^{-1}x = \cos^{-1}(2x^2-1)$
- $3\cos^{-1}x = \cos^{-1}(4x^3 -3x)$

<div>
$$
2 \tan^{-1}x = \tan^{-1}\Big(\frac{2x}{1-x^2}\Big) \\ 3\tan^{-1}x = \tan^{-1}\Big(\frac{3x-x^2}{1-3x^2}\Big)
$$
</div>

**Property 10**

$$
2\tan^{-1}x = \begin{cases}\sin^{-1}\Big(\frac{2x}{1+x^2}\\\cos^{-1}\Big(\frac{1-x^2}{1+x^2}\Big)\Big)\end{cases}
$$

$1-\cos\theta = 2 \sin^2(\theta/2)$

$1+ \cos\theta = 2\,\cos^2(\theta/2)$

$\sin\theta = 2\sin(\theta/2)\cos(\theta/2)$

$2\sin^{-1}x + \sin^{-1}(-x) = \cos^{1}x$

<div>
$$
\begin{split}\cos2\theta &= \cos^2\theta - \sin^2\theta \\& = 2\cos^2\theta -1 \\ &= 1 - 2\sin^2\theta \end{split}
$$
</div>

{{< panel title="Expression and Substitution" >}}

| Expression | Substitution | Substitution |
| --- | --- | --- |
| $a^2 + x^2$ | $x = a\tan\theta$ | $x = a\cot\theta$ |
|$a^2-x^2$ | $x=a\sin\theta$ | $x=a\cos\theta$ |
|$x^2-a^2$ | $x=a\sec\theta$ | $x=a\cosec\theta$ |
|$\frac{a-x}{a+x}$ | $x=a\cos2\theta$ | |
|$\frac{a^2+x^2}{a^2-x^2}$ | $x=a^2\cos2\theta$ |  |
{{< /panel >}}

## Line Equations

1. $ax + by + c=0$
    
    $m = -a/b$
        
2. One Point form of line 
    
    $$
    y - y_1 = m (x-x_1)
    $$
    
3. Two point form of line
    
    $$
    y-y_1 = \frac{y_2-y_1}{x_2-x_1}{x-x_1}
    $$
    
4. Intercept Form of line

    $$
    \frac{x}{a} + \frac{y}{b} = 1
    $$

{{< figure src="/images/etc/maths/Intercept_form.svg">}}

5. Normal form of line

    $$
    x\cos \theta + y\sin\theta = P
    $$

  {{< figure src="/images/etc/maths/Normal_Form.svg">}}

6. Point Slope form
    
    Where $m$ is slope of line defined as $m = \frac{y_2 - y_1}{x_2 - x_1}$
    

    $$
    y = mx+ c
    $$

    {{< figure src="/images/etc/maths/Point_SLope_form.svg">}}

### Distance of a point from a line

$$
\text{Dist}_{PA}= \Bigg|{\frac{ax_1 + by_1 + c}{\sqrt{a^2+b^2}}}\Bigg|
$$

{{< figure src="/images/etc/maths/distance_of_a_point_from_a_line.svg">}}

### Distance between two lines

$y = mx + c_1 \qquad y= mx+c_2$

$$
\text{d} = \Bigg| \frac{c_1 - c_2}{\sqrt{1+m^2}}\Bigg| = \Bigg|\frac{c_1 - c_2}{\sqrt{a^2+b^2}}\Bigg|
$$

### Angle between two lines

Where $m_1$ and $m_2$ are slopes of two lines.

$$
\tan\theta = \frac{m_2 - m_1}{1+m_2m_1}
$$

- If line $l_1$ and $l_2$ are orthogonal to each other, then. $m_1m_2 = -1$
- Collinearity of points
    
    Slope of $AB$ = Slope of $AC$

{{< figure src="/images/etc/maths/Collinearity.svg">}}

## Shapes CSA(Curved Surface Area), T(Total)SA, and volume

### Frustum

$\text{CSA} = \pi l (r_1+ r_2)$

$\text{TSA} = \pi r_1^2 + \pi r_2^2 + \pi l(r_1+r_2)$

$\text{Volume} = \frac{1}{3}\pi h (r_1^2 + r_2^2 + r_1r_2)$ 

where   $l= \sqrt{h^2+(r_1-r_2)^2}$

{{< figure src="/images/etc/maths/frustum.png">}}